KrakenStdlibCandidates/Init/All.lean
@@ -1,0 +1,15 @@
+prelude
+import KrakenStdlibCandidates.Init.Data.BitVec.Lemmas
+import KrakenStdlibCandidates.Init.Data.Nat.Lemmas
+import KrakenStdlibCandidates.Init.Data.Fin.Lemmas
+import KrakenStdlibCandidates.Init.Data.UInt8.Lemmas
+import KrakenStdlibCandidates.Init.Data.UInt16.Lemmas
+import KrakenStdlibCandidates.Init.Data.UInt32.Lemmas
+import KrakenStdlibCandidates.Init.Data.UInt64.Lemmas
+import KrakenStdlibCandidates.Init.Data.USize.Lemmas
+import KrakenStdlibCandidates.Init.Data.Int8.Lemmas
+import KrakenStdlibCandidates.Init.Data.Int16.Lemmas
+import KrakenStdlibCandidates.Init.Data.Int32.Lemmas
+import KrakenStdlibCandidates.Init.Data.Int64.Lemmas
+import KrakenStdlibCandidates.Init.Data.Int.Lemmas
+import KrakenStdlibCandidates.Init.Data.ISize.Lemmas
