KrakenStdlibCandidates/Init/Data/BitVec/Basic.lean
@@ -1,0 +1,32 @@
+prelude
+import Lean
+
+
+/-!
+# Basic definitions for BitVec.
+-/
+
+namespace BitVec
+
+def unsigned {w} (x : BitVec w) := Int.ofNat x.toNat
+
+theorem unsigned_append {n m : Nat} (a : BitVec n) (b : BitVec m) :
+    (a ++ b).unsigned = a.unsigned * (2 ^ m) + b.unsigned := by
+  dsimp only [unsigned]
+  rw [BitVec.toNat_append]
+  have hb := b.isLt
+  have h := (Nat.shiftLeft_add_eq_or_of_lt hb a.toNat)
+  rw [← h, Nat.shiftLeft_eq]
+  simp
+
+abbrev signed {w} (x : BitVec w) := x.toInt
+
+def take {w} (x : BitVec w) (n : Nat) : BitVec n := x.extractLsb' 0 n
+def drop {w} (x : BitVec w) (n : Nat) : BitVec (w - n) := x.extractLsb' n (w-n)
+
+def replaceLow {w n} (old : BitVec w) (new : BitVec n) : BitVec w :=
+  (BitVec.append (old.drop n) new).setWidth _
+def replace {w1} (old : BitVec w1) (i : Nat) {w2} (new : BitVec w2) : BitVec w1 :=
+  (old.drop (i + w2) ++ new ++ old.take i).setWidth _
+
+end BitVec
