KrakenStdlibCandidates/Init/Data/ISize/Lemmas.lean
@@ -1,0 +1,55 @@
+prelude
+import KrakenStdlibCandidates.Init.GrindInternHooks
+import KrakenStdlibCandidates.Init.Data.Int.Bitwise.Lemmas
+import KrakenStdlibCandidates.Init.Data.BitVec.Lemmas
+import KrakenStdlibCandidates.Init.Data.USize.Lemmas
+
+
+/-!
+# Grind homomorphism lemmas for ISize.
+-/
+
+attribute [grind_homo] ISize.toBitVec_add
+attribute [grind_homo] ISize.toBitVec_sub
+attribute [grind_homo] ISize.toBitVec_mul
+attribute [grind_homo] ISize.toBitVec_div
+attribute [grind_homo] ISize.toBitVec_mod
+attribute [grind_homo] ISize.toBitVec_and
+attribute [grind_homo] ISize.toBitVec_or
+attribute [grind_homo] ISize.toBitVec_xor
+attribute [grind_homo] ISize.toBitVec_shiftLeft
+attribute [grind_homo] ISize.toBitVec_shiftRight
+attribute [grind_homo] ISize.toBitVec_toInt8
+attribute [grind_homo] ISize.toBitVec_toInt16
+attribute [grind_homo] ISize.toBitVec_toInt32
+attribute [grind_homo] ISize.toBitVec_toInt64
+attribute [grind_homo] ISize.toBitVec_toUSize
+attribute [grind_homo] ISize.eq_iff_toBitVec_eq
+attribute [grind_homo] ISize.toBitVec_zero
+attribute [grind_homo] ISize.toBitVec_one
+attribute [grind_homo] ISize.toBitVec_not
+attribute [grind_homo] ISize.toBitVec_neg
+attribute [grind_homo] ISize.toBitVec_ofNat
+
+
+namespace ISize
+
+@[grind_homo] theorem toInt_eq_toBitVec_signed (x : ISize) : x.toInt = x.toBitVec.signed := rfl
+
+@[grind_homo_pred]
+theorem toBitVec_le (a b : ISize) : ISize.le a b ↔ (a.toBitVec.sle b.toBitVec = true) := Iff.rfl
+
+@[grind_homo_pred]
+theorem toBitVec_lt (a b : ISize) : ISize.lt a b ↔ (a.toBitVec.slt b.toBitVec = true) := Iff.rfl
+
+theorem toBitVec_injective : Function.Injective ISize.toBitVec := fun ⟨_⟩ ⟨_⟩ h => by congr; exact USize.toBitVec_injective h
+attribute [grind inj] toBitVec_injective
+
+@[grind_homo] theorem toBitVec_ofUSize (a : USize) : (ISize.ofUSize a).toBitVec = a.toBitVec := rfl
+
+@[grind_homo] theorem testBit_toBitVec (x : ISize) (i : Nat) :
+  x.toInt.testBit i = if i < System.Platform.numBits then x.toBitVec.getLsbD i else x.toBitVec.getLsbD (System.Platform.numBits - 1) :=
+  BitVec.testBit_toInt System.Platform.numBits_pos x.toBitVec i
+
+end ISize
+
