KrakenStdlibCandidates/Init/Data/Nat/Lemmas.lean
@@ -1,0 +1,5 @@
+import Init.Grind
+import KrakenStdlibCandidates.Init.GrindInternHooks
+
+@[grind_homo] theorem Nat.hShiftLeft_eq (a n : Nat) : a <<< n = a * 2^n := Nat.shiftLeft_eq a n
+@[grind_homo] theorem Nat.hShiftRight_eq (a n : Nat) : a >>> n = a / 2^n := Nat.shiftRight_eq_div_pow a n
