KrakenStdlibCandidates/Test/GrindHomoSharing.lean
@@ -1,0 +1,57 @@
+import KrakenStdlibCandidates
+import Init.Grind
+open Lean.Grind in #remove_toint_instances
+
+example (x0 : UInt8) :
+    let x := x0.toUInt16
+    let x := x + x
+    let x := x + x
+    let x := x + x
+    let x := x + x
+    let x := x + x
+    let x := x + x
+    let x := x + x
+    let x := x + x
+    x.toNat = x0.toNat*2^8 :=
+    by grind
+
+example (x0 : UInt16) :
+    let x := x0.toUInt32
+    let x := x + x
+    let x := x + x
+    let x := x + x
+    let x := x + x
+    let x := x + x
+    let x := x + x
+    let x := x + x
+    let x := x + x
+    x.toNat = x0.toNat*2^8 :=
+    by grind
+
+example (x0 : UInt32) :
+    let x := x0.toUInt64
+    let x := x + x
+    let x := x + x
+    let x := x + x
+    let x := x + x
+    let x := x + x
+    let x := x + x
+    let x := x + x
+    let x := x + x
+    x.toNat = x0.toNat*2^8 :=
+    by grind
+
+example (x0 : UInt16) :
+    let x := x0.toUSize
+    let x := x + x
+    let x := x + x
+    let x := x + x
+    let x := x + x
+    let x := x + x
+    let x := x + x
+    let x := x + x
+    let x := x + x
+    x.toNat = x0.toNat*2^8 := by
+  grind
+
+-- 16 doublings times out
