KrakenStdlibCandidates/Test/USizeCasesTest.lean
@@ -1,0 +1,5 @@
+import KrakenStdlibCandidates
+open Lean.Grind in #remove_toint_instances
+
+example (x : USize) : x.toNat >>> 64 = 0 := by
+  grind
