KrakenStdlibCandidates/tests/elab/test_instance_removal.lean
@@ -1,0 +1,13 @@
+import KrakenStdlibCandidates.Init.GrindInternHooks
+open Lean.Grind
+
+#remove_toint_instances
+
+/--
+error: failed to synthesize
+  ToInt.Add Nat (IntInterval.ci 0)
+
+Hint: Additional diagnostic information may be available using the `set_option diagnostics true` command.
+-/
+#guard_msgs in
+#synth ToInt.Add Nat (.ci 0)
